src/extra.v
@@ -118,3 +118,10 @@ Qed.
 Lemma big_sepM_imap {PROP : bi} `{Countable K} {A B} (f : K → A → B) (Φ : K → B → PROP) (m : gmap K A) :
   ([∗ map] k↦y ∈ map_imap (λ (k : K) a, Some (f k a)) m, Φ k y) ⊣⊢ ([∗ map] k↦y ∈ m, Φ k (f k y)).
 Proof. Admitted.
+
+Lemma big_sepM_impl' {PROP : bi} `{Countable K} {A B} (Φ : K → A → PROP) (Ψ : K → B → PROP) (m1 : gmap K A) (m2 : gmap K B) :
+  dom (gset K) m1 = dom _ m2 →
+  ([∗ map] k↦x ∈ m1, Φ k x) -∗
+  □ (∀ (k : K) (x : A) (y : B), ⌜m1 !! k = Some x⌝ → ⌜m2 !! k = Some y⌝ → Φ k x -∗ Ψ k y) -∗
+  [∗ map] k↦y ∈ m2, Ψ k y.
+Proof. Admitted.
